floyd/hints.v
@@ -1,0 +1,90 @@
+Require Import VST.floyd.base2.
+Require Import VST.floyd.client_lemmas.
+Require Import VST.floyd.go_lower.
+Require Import VST.floyd.closed_lemmas.
+Require Import VST.floyd.forward_lemmas VST.floyd.call_lemmas.
+Require Import VST.floyd.extcall_lemmas.
+Require Import VST.floyd.nested_field_lemmas.
+Require Import VST.floyd.efield_lemmas.
+Require Import VST.floyd.type_induction.
+Require Import VST.floyd.mapsto_memory_block.
+Require Import VST.floyd.data_at_rec_lemmas.
+Require Import VST.floyd.field_at.
+Require Import VST.floyd.loadstore_mapsto.
+Require Import VST.floyd.loadstore_field_at.
+Require Import VST.floyd.stronger.
+Require Import VST.floyd.local2ptree_denote.
+Require Import VST.floyd.local2ptree_eval.
+Require Import VST.floyd.reptype_lemmas.
+Require Import VST.floyd.proj_reptype_lemmas.
+Require Import VST.floyd.replace_refill_reptype_lemmas.
+Require Import VST.floyd.aggregate_type.
+Require Import VST.floyd.entailer.
+Require Import VST.floyd.globals_lemmas.
+Import Cop.
+Import Cop2.
+
+Ltac print_hint_forward c :=
+match c with
+| Ssequence ?c1 _ => print_hint_forward c1
+| Scall _ _ _ => idtac "Hint: try 'forward_call x', where x is a value to instantiate the tuple of the function's WITH clause"
+| Swhile _ _ => idtac "Hint: try 'forward_while'"
+| Sifthenelse _ _ _ => idtac "Hint: try 'forward_if'"
+| Sloop _ _ => idtac "Hint: try 'forward_loop' or 'forward_for_simple_bound'"
+| Sfor _ _ _ _ => idtac "Hint: try 'forward_loop' or 'forward_for_simple_bound'"
+| _ => idtac "Hint: try 'forward'"
+end.
+
+Ltac print_hint_semax D Pre c Post :=
+ try match Pre with exp _ => idtac "Hint: try 'Intros x' where x is the name you want to give the variable bound by EX'"  end;
+ try match Pre with PROPx (_::_) _ => idtac "Hint: use 'Intros' to move propositions above the line" end;
+ try match Pre with PROPx nil (LOCALx _ (SEPx _)) =>
+     let x := fresh "x" in
+      tryif (try (Intro x; fail 1)) then fail
+      else idtac "Hint: try 'Intros y' where y is the name you want to give the variable bound by EX'"
+     end;
+ try match Pre with PROPx nil (LOCALx _ (SEPx _)) =>
+     tryif (try (progress Intro_prop; fail 1)) then fail
+     else idtac "Hint: try 'Intros' to canonicalize your precondition"
+   end;
+ try match Pre with context [if ?A then _ else _] => 
+        match type of A with
+        | sumbool _ _ => idtac "Hint: perhaps  try 'destruct " A "' or, more concisely,  'if_tac'"
+        | bool => idtac "Hint: perhaps try 'destruct " A " eqn:?'"
+       end end;
+ try match Pre with PROPx nil (LOCALx _ (SEPx _)) => print_hint_forward c end;
+ idtac.
+
+Ltac hint :=
+ tryif (try (assert True; [ | solve [auto]]; fail 1)) then idtac
+     else  idtac "Hint:  'auto' solves the goal";
+ tryif (try (assert True; [ | solve [contradiction]]; fail 1)) then idtac
+     else  idtac "Hint:  'contradiction' solves the goal";
+ tryif (try (assert True; [ | discriminate]; fail 1)) then idtac
+     else  idtac "Hint:  'discriminate' solves the goal";
+ tryif (try (assert True; [ | solve [rep_omega]]; fail 1)) then idtac
+     else  idtac "Hint:  'rep_omega' solves the goal";
+ tryif (try (assert True; [ | progress entailer!]; fail 1)) then idtac
+     else  idtac "Hint:  try 'entailer!'";
+ tryif (try (progress autorewrite with sublist; fail 1)) then idtac
+     else  idtac "Hint:  try 'autorewrite with sublist'";
+ try match goal with |- _ |-- exp _ => idtac "Hint: try 'Exists x' where x is the value to instantiate the existential" end;
+ try match goal with H: ?p = nullval |- _ => idtac "Hint: try 'subst " p "'" end;
+ try match goal with |- ?A |-- ?B =>
+          tryif (try (assert True; [ | rewrite ?sepcon_emp, ?emp_sepcon; progress cancel]; fail 1)) then idtac
+           else  idtac "Hint:  try 'cancel'"
+       end;
+ try match goal with |- _ |-- ?B =>
+    match B with context [@exp _ _ ?t ] =>
+       idtac "Hint: try 'Exists x', where x is a value of type " t
+   end
+  end;
+ lazymatch goal with
+ | D := @abbreviate tycontext _, Po := @abbreviate ret_assert _ |- semax ?D' ?Pre ?c ?Post =>
+     constr_eq D D'; constr_eq Po Post; print_hint_semax D Pre c Post
+ | |- semax _ _ _ _ => 
+         idtac "Hint: use abbreviate_semax to put your proof goal into a more standard form"
+ | |- ENTAIL _, _ |-- _ => idtac "Hint: try 'entailer!'"
+ | |- _ => idtac
+ end.
+
