floyd/library.v
@@ -64,27 +64,29 @@ Parameter body_exit:
        {| sig_args := AST.Tint :: nil; sig_res := None; sig_cc := cc_default |})
    exit_spec'.
 
-Parameter malloc_token : share -> Z -> val -> mpred.
+Parameter malloc_token : forall {cs: compspecs}, share -> type -> val -> mpred.
 Parameter malloc_token_valid_pointer:
-  forall sh n p, malloc_token sh n p |-- valid_pointer p.
+  forall {cs: compspecs} sh t p, malloc_token sh t p |-- valid_pointer p.
 Hint Resolve malloc_token_valid_pointer : valid_pointer.
 Parameter malloc_token_local_facts:
-  forall sh n p, malloc_token sh n p |-- !! malloc_compatible n p.
+  forall {cs: compspecs} sh t p, malloc_token sh t p |-- !! malloc_compatible (sizeof t) p.
 Hint Resolve malloc_token_local_facts : saturate_local.
 Parameter malloc_token_precise:
-  forall sh n p, predicates_sl.precise (malloc_token sh n p).
+  forall {cs: compspecs} sh t p, predicates_sl.precise (malloc_token sh t p).
 
 Definition malloc_spec' :=
-   WITH n:Z
+   WITH cs: compspecs, t:type
    PRE [ 1%positive OF tuint ]
-       PROP (0 <= n <= Int.max_unsigned)
-       LOCAL (temp 1%positive (Vint (Int.repr n)))
+       PROP (0 <= sizeof t <= Int.max_unsigned;
+                complete_legal_cosu_type t = true;
+                natural_aligned natural_alignment t = true)
+       LOCAL (temp 1%positive (Vint (Int.repr (sizeof t))))
        SEP ()
     POST [ tptr tvoid ] EX p:_,
        PROP ()
        LOCAL (temp ret_temp p)
        SEP (if eq_dec p nullval then emp
-            else (malloc_token Tsh n p * memory_block Tsh n p)).
+            else (malloc_token Tsh t p * data_at_ Tsh t p)).
 
 Definition malloc_spec (prog: program) :=
    try_spec prog "_malloc" malloc_spec'.
@@ -95,11 +97,11 @@ Parameter body_malloc:
   body_lemma_of_funspec EF_malloc malloc_spec'.
 
 Definition free_spec' :=
-   WITH p:_, n:_
+   WITH cs: compspecs, t: type, p:val
    PRE [ 1%positive OF tptr tvoid ]
        PROP ()
        LOCAL (temp 1%positive p)
-       SEP (malloc_token Tsh n p; memory_block Tsh n p)
+       SEP (malloc_token Tsh t p; data_at_ Tsh t p)
     POST [ Tvoid ]
        PROP ()
        LOCAL ()
@@ -125,13 +127,13 @@ Ltac with_library prog G :=
  with_library' prog y.
 
 Lemma semax_func_cons_malloc_aux:
-  forall (gx : genviron) (x : Z) (ret : option val),
+  forall {cs: compspecs} (gx : genviron) (t :type) (ret : option val),
 (EX p : val,
  PROP ( )
  LOCAL (temp ret_temp p)
  SEP (if eq_dec p nullval
       then emp
-      else malloc_token Tsh x p * memory_block Tsh x p))%assert
+      else malloc_token Tsh t p * data_at_ Tsh t p))%assert
   (make_ext_rval gx ret) |-- !! is_pointer_or_null (force_val ret).
 Proof.
  intros.
