floyd/proofauto.v
@@ -37,6 +37,7 @@ Require Export VST.floyd.globals_lemmas.
 Require Export VST.floyd.diagnosis.
 Require Export VST.floyd.freezer.
 Require Export VST.floyd.deadvars.
+Require Export VST.floyd.hints.
 Require Export VST.floyd.Clightnotations.
 Arguments semax {CS} {Espec} Delta Pre%assert cmd%C Post%assert.
 Export ListNotations.
@@ -77,6 +78,15 @@ Hint Rewrite modu_repr using rep_omega : entailer_rewrite norm.
 
 Hint Rewrite Vptrofs_unfold_false using reflexivity: entailer_rewrite norm.
 Hint Rewrite Vptrofs_unfold_true using reflexivity: entailer_rewrite norm.
+
+Hint Rewrite @upd_Znth_app1 using list_solve : sublist.
+Hint Rewrite @upd_Znth_app2 using list_solve : sublist.
+
+Lemma map_list_repeat: forall {A B} (f: A->B) n (x:A), map f (list_repeat n x) = list_repeat n (f x).
+Proof.
+intros. induction n; simpl; f_equal; auto.
+Qed.
+Hint Rewrite @map_list_repeat : sublist.
 
 Arguments deref_noload ty v / .
 Arguments nested_field_array_type {cs} t gfs lo hi / .
